src/tactics/boot/FStar.Tactics.Interpreter.fs
@@ -511,7 +511,7 @@ let by_tactic_interp (pol:pol) (e:Env.env) (t:term) : tres =
     let hd, args = U.head_and_args t in
     match (U.un_uinst hd).n, args with
 
-    // by_tactic marker
+    // with_tactic marker
     | Tm_fvar fv, [(rett, Some (Implicit _)); (tactic, None); (assertion, None)]
             when S.fv_eq_lid fv PC.by_tactic_lid ->
         begin match pol with
@@ -529,7 +529,7 @@ let by_tactic_interp (pol:pol) (e:Env.env) (t:term) : tres =
         end
 
     // spinoff marker: simply spin off a query independently.
-    // So, equivalent to `by_tactic idtac` without importing the (somewhat heavy) tactics module
+    // So, equivalent to `with_tactic idtac` without importing the (somewhat heavy) tactics module
     | Tm_fvar fv, [(assertion, None)]
             when S.fv_eq_lid fv PC.spinoff_lid ->
         begin  match pol with
